# General Equation of Line

Different ways to represent a line.
| Representation | Equation |
| --- | --- |
|slope-intercept form | $(y-y_0)=m(x-x_0)$
|slope-point form| $y=mx+c$ or $y = m(x-d)$
|Two point form| $(y-y_1) = \frac{y_2-y_1}{x_2-x_1}(x-x_1)$
|Intercept form| $\frac{x}{a}+\frac{y}{b}=1$

General Equation of Line
| Representation | Equation |
| --- | --- |
| General form | $Ax+By+C=0$ |
| Point-slope form | $m = -\frac{A}{B},y_0=mx_0=-\frac{C}{B}$ |
| Slope-intercept form | $m=-\frac{A}{B},c=-\frac{C}{B}, d =-\frac{C}{A}$ |
| Two point form | $\frac{y_2-y_1}{x_2-x_1}=-\frac{A}{B},y_1+\frac{A}{B}x_1=-\frac{C}{B}$ |
| Intercept form | $a=-\frac{C}{A},b=-\frac{C}{B}$ |

Any equation of the form $Ax+By+C=0$ is called a **general equation of a line**. The line is called the **general line**. where $A,B\neq0$ simultaneously.

## Example

- [ ] Let the eqaution of a line be $3x-4y+12=0$. Find the slope and x-intercept and y-intercept of the line.
- Identified $A = 3, B = -4, C =12$
- Using Intercept form, $a = -\frac{C}{A} = -\frac{12}{3} = -4$ and $b = -\frac{C}{B} = -\frac{12}{-4} = 3$
- Using Slope-intercept form, $m = -\frac{A}{B} = -\frac{3}{-4} = \frac{3}{4}$
- Slope = $\frac{3}{4}$ and x-intercept = $4$ and y-intercept = $3$
- [ ] Show that the two lines $a_1x+b_1y+c=0$ and $a_2x+b_2y+c\neq0$
- The lines are parallel if $a_1b_2=a_2b_1$ and $a_1b_2\neq0$
- The lines are perpendicular if $a_1a_2+b_1b_2=0$
- Using Slope Intercept form, $m_1 = -\frac{a_1}{b_1}$ and $m_2 = -\frac{a_2}{b_2}$
- [ ] Find the equation of a line which is perpendicular to the line $x-2y+3=0$ and passes through the point $(-1,2)$
- $m_1 = -\frac{A}{B} = -\frac{1}{-2}$ = $\frac{1}{2}$
- The slope of the perpendicular line is $m_2 = -\frac{1}{m_1} = -\frac{1}{\frac{1}{2}} = -2$
- The equation of the perpendicular line is
  - $(y-2) = -2(x - (-1))$
  - $y = -2x -2 + 2$
  - $y = -2x$
- [ ] The equation of a line passing through the point $(3,4)$ and perpendicular to the line $3x + 4y âˆ’ 8 = 0$ is
- $m_1 = -\frac{A}{B} = -\frac{3}{4}$
- $m_2 = -\frac{1}{m_1} = -\frac{1}{-\frac{3}{4}} = \frac{4}{3}$
- $(y-4) = \frac{4}{3}(x-3)$
- $3(y-4) = 4(x-3)$
- $3y - 12 = 4x - 12$
- $3y = 4x$
- $0 = 4x - 3y$
- multiplying by 2
- $0 = 8x - 6y$
