# Alebra on Polynomials

## Addition

- The formula for adding two polynomials are:

  - $p(x)+q(x) = \sum^{m \vee n}_{k=0}(a_k+b_k)x^k$

- [ ] $p(x)= x^2=4x+4, q(x) = 10$

  - $p(x)+q(x)=x^2+4x+4+10$
  - $p(x)+q(x)=x^2+4x+14$

- [ ] $p(x)=x^4+4x, q(x)=x^3+1$

  - $p(x)+q(x)=x^4+4x+x^3+1$
  - $p(x)+q(x)=x^4+x^3+4x+1$

- [ ] $p(x)=x^3+2x^2+1, q(x)=x^2+2x+2$
  - $p(x)+q(x)=x^3+2x^2+1+x^2+2x+2$
  - $p(x)+q(x)=x^3+x^2+2x^2+2x+1+2$
  - $p(x)+q(x)=x^3+x^2+2x^2+2x+3$

---

## Subtraction

- The formula for adding two polynomials are:

  - $p(x)+q(x) = \sum^{m \vee n}_{k=0}(a_k - b_k)x^k$

- [ ] $p(x)=x^2+4x+4, q(x)=10$

  - $p(x)-q(x)=x^2+4x+4-10$
  - $p(x)-q(x)=x^2+4x-6$

- [ ] $p(x)=x^4+4x, q(x)=x^3+1$

  - $p(x)-q(x)=x^4+4x-x^3-1$
  - $p(x)-q(x)=x^4-x^3+4x-1$

- [ ] $p(x)=x^3+2x^2+1, q(x)=x^2+2x+2$

  - $p(x)-q(x)=x^3+2x^2+1-x^2-2x-2$
  - $p(x)-q(x)=x^3-x^2+2x^2-2x+1-2$
  - $p(x)-q(x)=x^3-x^2+2x^2-2x-1$

---

## Multiplication

- The formula for multiplying two polynomials are:

  - $p(x)q(x) = \sum^{m+n}_{k=0}\sum^{k}_{j=0}a_ix^ib_{k-j}x^k$

- [ ] $p(x)= (x^2+x+1), q(x)=(2x^3)$
  - $p(x)q(x) = (x^2+x+1)(2x^3)$
  - $p(x)q(x) = 2x^5+2x^4+x^3+x^2+x$
- [ ] $p(x)= x^2+x+1, q(x)=x^2+2x+1$

---

## Division

- The formula for dividing
  - Arrange the polynomials in descending order and add the missing exponent with 0 coefficient.
  - Divide the first term of the dividend by the first term of the divisor and we get a monomial.
  - Multiply the monomial with the divisor and subtract it from the dividend.
  - Check if the resulatant polynomial has a degree less than the divisor. If true then the division is complete and write the polynomial as the remainder. If not then go to step 2.

### Example

- [ ] $p(x)=\frac{3x^2+x+3}{x}$
  - $\frac{x(3x+1)+3}{x}$
  - $3x+1+\frac{3}{x}$
- [ ] $p(x)=\frac{3x^2+x+1}{x+1}$
  - $\frac{3x^2+4x+1}{x+1}$
  - Divide the terms in pair
  - $=3x+1$
- [ ] $p(x) = \frac{2x^3+3x^2+1}{2x+1}$
  - Dividing using long division
    - $\phantom{asdfas}x^2+x-\frac{1}{2}$
    - $2x+1\overline{)2x^3+3x^2+0x+1}$
    - $\phantom{asd}-(2x^3+x^2)$
    - $\phantom{asdfaa}\overline{0 \ \ + \  2x^2+0x+1}$
    - $\phantom{asdasdfs}-(2x^2+x)$
    - $\phantom{asdfaa}\overline{0 \ \ + \ \ \ \ 0 \ -1x+1}$
    - $\phantom{asdasdfsasdfa}-(1x+\frac{1}{2})$
    - $\phantom{asdasdfsasdfa} \ \ \ \ \ \overline{\frac{3}{2} \ \ \ \ \ \  \ \ \ \ \ \ \ \ }$
    - Therefore the quotient is $x^2+x-\frac{1}{2}$ and the remainder is $\frac{3}{2}$
