# Second order partial derivatives for $f(x,y)$

- Let $f(x,y)$ be a function of two variables.
- Then the second order partial derivatives for $f$ are the partial derivatives of the first order partial derivatives.
- $$
  \begin{align} f_{xx} &=(fx)x &= \frac{\partial^2 f}{\partial x^2}
  \\ f_{xy} &=(fx)y &= \frac{\partial^2 f}{\partial y \partial x}
  \\ f_{yx} &=(fy)x &= \frac{\partial^2 f}{\partial x \partial y}
  \\ f_{yy} &=(fy)y &= \frac{\partial^2 f}{\partial y^2} \end{align}
  $$

### Example

- $f(x,y) = x+y$
  - $\frac{\partial f}{\partial x} = 1$
  - $\frac{\partial f}{\partial y} = 1$
  - $f_{xx} = \frac{\partial^2 f}{\partial x^2} = 0$
  - $f_{xy} = \frac{\partial^2 f}{\partial y \partial x} = 0$
- $f(x,y) = sin(xy)$
  - $\frac{\partial f}{\partial x} = y\cos(xy)$
  - $\frac{\partial f}{\partial y} = x\cos(xy)$
  - $f_{xx} = \frac{\partial^2 f}{\partial x^2} = -y^2\sin(xy)$
  - $f_{xy} = \frac{\partial^2 f}{\partial y \partial x} = -xy\sin(xy)$
  - $f_{yx} = \frac{\partial^2 f}{\partial x \partial y} = -yx\sin(xy)$
  - $f_{yy} = \frac{\partial^2 f}{\partial y^2} = -x^2\sin(xy)$

## Clairaut's Theorem

- Let $f(x,y)$ be a function defined on a domain in $D$ in $\mathbb{R}^2$ containing some open ball around the point $a$.
- If the second order partial derivatives $f_{xy}$ or $f_{yx}$ are continuous on some open ball around the point $a$ then $f_{xy} = f_{yx}$.

# Higher order partial derivatives

- Let $f(x_1,x_2, \dots, x_n)$ be a function defined on a domain D in $\mathbb{R}^n$. Then the higher order partial derivatives of $f$ are defined by taking successive partial derivatives of $f$.
  $$ f_{x_1x_2 \dots x_n} = \frac{\partial^4 f}{\partial x_1 \partial x_2 \dots \partial x_n} $$
- An appropriately modified statement of Clairaut's theorem holds.

# Hessian matrix

- Let $f(x_1,x_2, \dots, x_n)$ be a function defined on a domain D in $\mathbb{R}^n$.
- Then the Hessian matrix of $f$ is defined has
  $$\begin{bmatrix} f_{xx} & f_{xy} & \dots & f_{x_n} \\ f_{yx} & f_{yy} & \dots & f_{y_n} \\ \vdots & \vdots & \ddots & \vdots \\ f_{n_1x} & f_{n_1y} & \dots & f_{n_1n} \end{bmatrix}$$

### Example

- $f (x,y,z) = xy + yz + xz$
  - $\begin{bmatrix} f_{xx} & f_{xy} & f_{xz} \\ f_{yx} & f_{yy} & f_{yz} \\ f_{zx} & f_{zy} & f_{zz} \end{bmatrix} = \begin{bmatrix} 0 & 1 & 1 \\ 1 & 0 & 1 \\ 1 & 1 & 0 \end{bmatrix}$
