# Quadratic Equation: Intercept Form

- Let $y=f(x)=(x-p)(x-q)$, where $p$ and $q$ are represent x-intercepts for the function. Then they form $y = a(x-p)(x-q)$ is called the intercept form of the quadratic equation.

- Example: Graph $y=3(x-1) (x-5)$
- In this graph the x = 1 and x = 5 are the x-intercepts.
- The axis of symmetry is $x$ is the average of the x-intercepts, which is $x = \frac{1+5}{2} = 3$.
- The vertex is $3(3-1)(3-5) = 3(2)(-2) = -12$.
- Vertex: $(3,-12)$

# Intercept Form to Standard Form

- Changing intercept form to standard form requires us to use the FOIL method.
  - The product of the first **(F)** terms, the product of the outer **(O)** terms, the product of the inner **(I)** terms, and the product of the last **(L)** terms.
  - $(ax+b)(cx+d)= ax.cx+ax.d+b.cx+b.d$
    - Quick Overvation:
      - The product of coefficients is $ac$ and the product of the constants is $bd$ is $abcd$.
      - Thr product of the two terms in the coeffiecient of $x$ is also $abcd$.

## Examples of FOIL Method

- Write the equation with roots $\frac{2}{3}$ and $-4$, in the standard form.
  - $y = (x-\frac{2}{3})(x+4)$
  - $y = x^2+ (-\frac{2}{3}+4)x -\frac{8}{3}=x^2+\frac{10}{3}x-\frac{8}{3}$
  - $x^2 + \frac{10}{3}x - \frac{8}{3} = 0$
  - Multiplying both sides by 3
  - $3x^2 + 10x - 8 = 0$

## Standard Form to Intercept Form
- Convert the function $f(x) = 5x^2-13x+6$ to intercept form.
- Let us apply the FOIL method to the function.
  - $f(x) = 5x^2-13x+6$
  - $f(x) = 5x.5x-13x.5+6.5$
  - $f(x) = 25x^2-65x+30$
  - $f(x) = (x-2)(x-15)$
