# Integrals

## Basic Properties of Integrals

- The integral of a constant is the constant times the variable
  $$\int c f(x)dx = c\int f(x)dx $$
- The integral of a sum is the sum of the integrals
  $$\int (f(x) + g(x))dx = \int f(x)dx + \int g(x)dx$$
- The integral of a difference is the difference of the integrals
  $$\int (f(x) - g(x))dx = \int f(x)dx - \int g(x)dx$$
- The integral of a product is the product of the integrals
  $$\int (f(x)g(x))dx = \int f(x)dx \int g(x)dx$$

## Integration by Parts:

$$\int fg'(x) dx = (fg)(x)- \int(f'g)(x)dx$$

### Proof

- $\frac{d}{dx}(fg)(x) = f'(x)g(x)+g'(x) = (f'g)(x) + (g'f)(x)$
- $\int (f'g+g'f)(x) dx = (fg)(x)$
- $\int(f'g)(x)dx+\int(g'f)(x)dx = (fg)(x)$
- $\int(g'f)(x) dx= (fg)(x) - \int(f'g)(x)dx$

## Basic Properties of definite integrals

- The definite integral of a constant is the constant times the interval
  $$\int_a^b c f(x)dx = c\int_a^b f(x)dx $$
- The definite integral of a sum is the sum of the definite integrals
  $$\int_a^b (f(x) + g(x))dx = \int_a^b f(x)dx + \int_a^b g(x)dx$$
- The difference of the definite integrals
  $$\int_a^b (f(x) - g(x))dx = \int_a^b f(x)dx - \int_a^b g(x)dx$$
- To invert the order of integration
  $$\int_b^a f(x)dx = -\int_a^bf(x)dx$$
- For any constant $c \in \mathbb{R}$
  $$\int_a^bf(x)dx=\int_a^cf(x)dx+\int_a^cf(x)dx$$
- If $f(x) \geq g(x)$ for all byt finitely many points on the interval $[a,b]$
  $$\int_a^bf(x)dx \geq \int_a^bg(x)dx$$

## Integration of piecewise functions

- If $f$ is defined peicewise on subintervals of $[a,b]$ then it's definite integral from $a$ to $b$ can be computed by computing the definite integrals on each subinterval and adding them up.
- Example: $f(x) = \begin{cases} x & \text{if } 0  \leq x \leq 1  \\ 3x-1 &  \text{if } 1  \leq x \leq 2 \end{cases}$
- What is $\int_0^2 f(x) dx ?$
  $$\int_0^2f(x) dx = \int_0^1f(x)dx+\int_1^2f(x)dx$$
  $$\int_0^2f(x) dx = \int_0^1 x dx + \int_1^2 3x-1 dx$$
  $$\int_0^2f(x) dx = \frac{1}{2}x^2|_0^1 + \frac{1}{3}3x^3-3x|_1^2$$
  $$\int_0^2f(x) dx = \frac{1}{2} - \frac{1}{3} + \frac{1}{3}3 - \frac{1}{3} = \frac{1}{2}$$
  $$\int_0^2f(x) dx = 2$$

## Integration by Parts (definite integral)

- Formula:
  $$\int_a^b (fg')(x)dx = (fg)(b)-(fg)(a)-\int_a^b(f'g)(x)(dx)$$
- Example : $\int_0^\infty 3xe^{-2x} dx$
  - $f(x) = x$
  - $g'(x)=3e^{-3ex}$
  - $g(x) = \frac{3}{-3}e^{-3ex}= -e^{-3ex}$
  - $(x)e^{-3ex}dx|^b_0 - \int_0^b1\cdot (-e^{-3x})$
  - $(x)e^{-3ex}dx|^b_0 - \frac{e^{-3x}}{3}|^b_0$
  - $-be^{-3eb} - \frac{e^{-3x}}{3}|^b_0$
  - $-be^{-3eb} - (\frac{e^{-3b}}{3}-\frac{1}{3})$
  - $-be^{-3eb}-\frac{e^{-3b}}{3}+\frac{1}{3}$
  - As $b \to \infin$
  - $\frac{1}{3}$

## Integration by Substitution

- Formula:
  $$\int_a^b f(g(x))g'(x)dx = \int_{g(a)}^{g(a)} f(u)du$$
